---
title:
---

$$
∬_{x^{2}+y^{2} ⩽ 1} \sqrt[3]{\sin (x-y)}\, d x d y
$$

$$
\begin{aligned}
 I&=∬_{x^{2}+y^{2} ⩽ 1} \sqrt[3]{\sin (x-y)}\, d x d y\\
 &=∬_{x^{2}+y^{2} ⩽ 1} \sqrt[3]{\sin (y-x)}\, d y d x\\
 &=-I
\end{aligned}\\∴ I=0
$$

---

$$
∬_{x^{2} ⩽ 1, y^{2} ⩽ 1} \frac{a \mathrm{e}^{x}+b \mathrm{e}^{y}}{\mathrm{e}^{x}+\mathrm{e}^{y}} \,\mathrm{d} x \,\mathrm{d} y
$$

$$
\begin{aligned}
&=\frac 12\left(
 ∬_{x^{2} ⩽ 1, y^{2} ⩽ 1} \frac{a \mathrm{e}^{x}+b \mathrm{e}^{y}}{\mathrm{e}^{x}+\mathrm{e}^{y}} \,\mathrm{d} x \,\mathrm{d} y+
 ∬_{x^{2} ⩽ 1, y^{2} ⩽ 1} \frac{b \mathrm{e}^{x}+a \mathrm{e}^{y}}{\mathrm{e}^{x}+\mathrm{e}^{y}} \,\mathrm{d} x \,\mathrm{d} y
\right)\\
&=\frac {a+b}2 ∬_{x^{2} ⩽ 1, y^{2} ⩽ 1}\,\mathrm{d} x \,\mathrm{d} y\\
&=2(a+b)
\end{aligned}
$$

>[积分值与积分变量记号（名称）无关](http://blog.sina.com.cn/s/blog_{4}aa977290100g0zu.html)

---

$$
\begin{aligned}
&∫ x^{3} e^{x^{2}} \,dx\\
=&\frac 12∫ x^{2} e^{x^{2}} \,dx^{2}\\
=&\frac 12 \left(x^{2}-1\right)e^{x^{2}}+C
\end{aligned}
$$

---

$$
∬_{D} e^{x y} d x d y,D=\{(x, y) 1 ⩽ x y ⩽ 2, x ⩽ y ⩽ 2 x\}
$$

> $x ⩽ y ⩽ 2 x\impliesθ∈[\frac{π}4,\arctan 2]$
> 
> $1 ⩽ x y ⩽ 2=1 ⩽ ρ^{2}\sin θ\cos θ ⩽ 2⟹\frac{1}{\sqrt{\cos θ \sin θ}} ⩽ ρ ⩽ \sqrt{\frac{2}{\cos θ \sin θ}}$

$$
\begin{aligned}
 I&=∫_{\frac{π}{4}}^{\arctan 2} d θ ∫_{\frac{1}{\sqrt{\cos θ \sin θ}}}^{\sqrt{\frac{2}{\cos θ \sin θ}}} e^{ρ^{2} \sin θ \cos θ} ρ \,d ρ\\
 &=∫_{\frac{π}{4}}^{\arctan 2}\left[\left.\frac{1}{2} \frac{1}{\cos θ \sin θ} e^{ρ^{2} \cos θ \sin θ} \right| \sqrt{\frac{2}{\cos θ \sin θ}}\right]\, d θ\\
 &=∫_{\frac{π}{4}}^{\arctan 2} \frac{1}{2 \cos θ \sin θ}\left(e^{2}-1\right) \,d θ=\frac{e^{2}-e}{2} \ln 2
\end{aligned}
$$

---

$f(t)$ 连续，证
$$
∬_{|x|+|y| ⩽ 1} f(x+y) \,d x d y=∫_{-1}^{1} f(u)\, d u
$$

$$
\begin{cases}
x=\frac{u}{\sqrt{2}}-\frac{v}{\sqrt{2}} \\
y=\frac{u}{\sqrt{2}}+\frac{v}{\sqrt{2}}
\end{cases}
$$

$$
LHS=∫_{-\frac{\sqrt{2}}{2}}^{\frac{ \sqrt{2}}{2}}\, d v
∫_{-\frac{\sqrt{2}}{2}}^{\frac{\sqrt 2}{2}} f\left(\sqrt{2} u\right) \,d u\\
\sqrt 2u=t,du=dt/\sqrt 2,t :-1→ 1\\
=\sqrt{2} ∫_{-1}^{1} f(t) \frac{d t}{\sqrt{2}}=RHS
$$

>解法略超纲

---

$$
D:0 ⩽ θ ⩽ \frac {π}2,
0 ⩽ ρ ⩽ 1,
∬_{D}\sqrt{1-ρ^{2}} ρ\, d ρ d θ
$$

$$
\begin{aligned}
&∫_{0}^{\frac{π}{2}}\,dθ
∫_{0}^{1}{\sqrt{1-ρ ^{2}}ρ \,dρ }\\
=&-\frac 12 ∫_{0}^{\frac{π}{2}}\,dθ
∫_{0}^{1}{\sqrt{1-ρ ^{2}} \,d\left(1-ρ^{2}\right) }\\
=&\frac {π}6
\end{aligned}
$$

>$z=\sqrt{1-ρ^{2}}=\sqrt{1-\left(x^{2}+y^{2}\right)}⟹ x^{2}+y^{2}+z^{2}=1$
>其中 $x ⩾ 0,y ⩾ 0,z ⩾ 0$

---
