---
title:
---

$f(t)$ 在 $[0,1]$ 上连续，证

$$
∫_{0}^{1} d x ∫_{0}^{x} d y ∫_{0}^{y} f(x) f(y) f(z)\, d z=\frac{1}{3 !}\left[∫_{0}^{1} f(t)\, d t\right]^{3}
$$

令
$$
F(x)=∫_{0}^{x} f(t)\, d t,F(0)=0
$$

$$
\begin{aligned}
LHS&=∫_{0}^{1} f(x) d x ∫_{0}^{x} f(y) d y ∫_{0}^{y} f(z) d z\\
&=∫_{0}^{1} f(x) d x ∫_{0}^{x} f(y) d y (F(y)-F(0))\\
&=∫_{0}^{1} f(x) d x ∫_{0}^{x} f(y)F(y) d y\\
&=∫_{0}^{1} f(x) d x ∫_{0}^{x} F(y) d F(y)\\
&=∫_{0}^{1} f(x) \frac{1}{2}[F(x)]^{2} d x\\
&=\frac{1}{2}\frac{1}{3}[F(1)]^{3}=RHS
\end{aligned}
$$

---
