---
title: æœŸç»ˆï¼ˆä¸€ï¼‰
---

$Ï†(x)$ æœ‰ä¸‰é˜¶å¯¼æ•°ï¼Œ$Ï†(x_0)=0,Ï†'(x_0)â‰  0$ .è¯æ˜ $(x_0,0)$ æ˜¯ $y=(x-x_0)^2Ï†(x)$ çš„æ‹ç‚¹

é”™è¯¯åŸå› ï¼šåªæ±‚äº† $y''(x_0)=0$,è¦è®ºè¯ $y'''(x_0)$ çš„æƒ…å†µ

å‰ç•¥
$$
y'''(x) = 6 Ï† ' ( x ) + 6 \left( x - x _ { 0 } \right) Ï† '' ( x ) + \left( x - x _ { 0 } \right) ^ { 2 } Ï† ''' ( x )\\
y ''' \left( x _ { 0 } \right) = 6 Ï† ' \left( x _ { 0 } \right) â‰ q 0\\
y ''' \left( x _ { 0 } \right) = \lim _ { x â†’ x _ { 0 } } \frac { y '' ( x ) - y '' \left( x _ { 0 } \right) } { x - x _ { 0 } } = \lim _ { x â†’ x _ { 0 } } \frac { y '' ( x ) } { x - x _ { 0 } }
$$
å±€éƒ¨ä¿å·æ€§ï¼Œ$y'''(x_0)$ ä¸å˜å·ï¼Œ$âˆ´ y''(x)$ å˜å·ï¼Œæ‰€ä»¥æ˜¯æ‹ç‚¹

---

$$
âˆ« \frac{3 x^2-4 x+10}{x^3+8} \, \,\mathrm{d}x
$$

è®°å¾—ç”¨ç«‹æ–¹å’Œå…¬å¼ã€‚ã€‚ã€‚è¿™é¢˜æˆ‘å†™å¾—æ¯”ç­”æ¡ˆç®€æ´ğŸ˜
$$
\begin{aligned}
&= âˆ« \frac { 3 x ^ { 2 } - 4 x + 10 } { ( x + 2 ) \left( x ^ { 2 } - 2 x + 4 \right) } \,\mathrm{d}x\\
&= âˆ« \left( \frac { x } { 2 \left( x ^ { 2 } - 2 x + 4 \right) } + \frac { 5 } { 2 ( x + 2 ) } \right) \,\mathrm{d}x\\
&=1/2âˆ« \frac{\,\mathrm{d} (x-1)}{(x-1)^2+3}+5/2\ln|x+2|+C\\
&=\frac1{2\sqrt3} âˆ« \frac{\,\mathrm{d} \left(\frac{x-1}{\sqrt 3}\right)}{\left(\frac{x-1}{\sqrt 3}\right)^2+1}+5/2\ln|x+2|+C\\
&=\frac1{2\sqrt3}\arctan \left(\frac{x-1}{\sqrt 3}\right)+\frac52\ln|x+2|+C
\end{aligned}
$$

---

è®¾ $f(x)$ åœ¨ $[0,a]$ è¿ç»­ï¼Œè¯æ˜
$$
âˆ« _0^a f(x)\,\,\mathrm{d}x=âˆ« _0^a f(a-x)\,\,\mathrm{d}x
$$
å¹¶åˆ©ç”¨æ­¤å¼ï¼Œè®¡ç®—
$$
âˆ« _0^{\frac Ï€ 4} \frac{1-\sin 2x}{1+\sin 2x}\,\,\mathrm{d}x
$$

$$
âˆ« _0^a f(x)\,\,\mathrm{d}x \,\xlongequal {t = a - x} âˆ« _{a}^0 f(t)\,\mathrm{d} (-t)=-âˆ« _{a}^0 f(t)\,\mathrm{d} t=âˆ« _0^a f(t)\,\mathrm{d} t
$$

$$
\begin{aligned}
I &= âˆ« _ { 0 } ^ { \frac { Ï€ } { 4 } } \frac { 1 - \sin 2 x } { 1 + \sin 2 x }\, \,\mathrm{d}x\\
&= âˆ« _ { 0 } ^ { \frac { Ï€ } { 4 } } \frac { 1 - \sin \left[ 2 \left( \frac { Ï€ } { 4 } - x \right) \right] } { 1 + \sin \left[ 2 \left( \frac { Ï€ } { 4 } - x \right) \right] }\, \,\mathrm{d}x\\
&= âˆ« _ { 0 } ^ { \frac { Ï€ } { 4 } } \frac { 1 - \cos 2 x } { 1 + \cos 2 x } \,\,\mathrm{d}x\\
&= âˆ« _ { 0 } ^ { \frac { Ï€ } { 4 } } \frac { 2 \sin ^ { 2 } x } { 2 \cos ^ { 2 } x } \,\mathrm{d}x \\
&= âˆ« _ { 0 } ^ { \frac { Ï€ } { 4 } } \tan ^ { 2 } x \,\mathrm{d}x \\
&= âˆ« _ { 0 } ^ { \frac { Ï€ } { 4 } } \left( \sec ^ { 2 } x - 1 \right) \,\mathrm{d}x = 1 - \frac { Ï€ } { 4 }
\end{aligned}
$$

---