---
title: 自测题13
---

$$
∫ \frac{\sin x\cos x}{\sqrt{a^2\sin^2x+b^2\cos^2 x}}{\rm d}x
$$

$u=a^2 \sin ^2(x)+b^2 \cos ^2(x)$

${\rm d}u=2 a^2 \sin (x) \cos (x)-2 b^2 \sin (x) \cos (x){\rm d}x$

$a≠ b$时
$$
\begin{aligned}
LHS&=\frac{1}{2 \left(a^2-b^2\right)}∫ \frac{1}{\sqrt{u}} {\rm d}u\\
&=\frac{\sqrt{u}}{a^2-b^2}+C\\
&=\frac{\sqrt{a^2 \sin ^2(x)+b^2 \cos ^2(x)}}{a^2-b^2}+C
\end{aligned}
$$

$a=b$时
$$
\begin{aligned}
LHS&=\frac{1}{|a|}∫\frac{\sin x\cos x}{\sqrt{\sin^2x+\cos^2 x}}{\rm d}x\\
&=\frac{1}{2|a|}∫\sin 2x {\rm d}x\\
&=-\frac{\cos ^2x}{2 |a|}
\end{aligned}
$$

---

$$
∫ \cot ^6(x) \sec ^3(x) {\rm d}x=\frac { \csc ^ { 3 } ( x ) } { 3 } - \frac { \csc ^ { 5 } ( x ) } { 5 }+C
$$
开始的消项是关键
$$
\begin{aligned}
∫ \left( \cot ^3x\right) \left( \csc ^3x\right) {\rm d}x&=∫ (\cot x) \left(\csc ^3x\right) \left(\csc ^2x-1\right) {\rm d}x\\
\color{red} u&\color{red}= \csc x\quad {\rm d} u = - \cot ( x ) \csc ( x ) {\rm d} x\\
&=- ∫ u ^ { 2 } \left( u ^ { 2 } - 1 \right) {\rm d} u\\
&= \frac { u ^ { 3 } } { 3 } - \frac { u ^ { 5 } } { 5 }\\
&= \frac { \csc ^ { 3 } ( x ) } { 3 } - \frac { \csc ^ { 5 } ( x ) } { 5 }+C\\
\end{aligned}
$$

---

$$
∫ \frac{2^x 3^x}{9^x+4^x}{\rm d}x
$$

$$
LHS= ∫ \frac { \left( \frac { 2 } { 3 } \right) ^ { x } } { 1 + \left( \frac { 2 } { 3 } \right) ^ { 2x } } {\rm d} x \quad 此处同除4^x也行\\
t=\left( \frac { 2 } { 3 } \right) ^ { x },x=\log_{\frac { 2 } { 3 }}t,{\rm d}x=\frac 1{t\ln\frac { 2 } { 3 }}{\rm d}t\\
\begin{aligned}
LHS
&=∫ \frac { t } { 1 +t^2 }⋅ \frac 1{t\ln\frac { 2 } { 3 }}{\rm d}t\\
&=\frac 1{\ln\frac { 2 } { 3 }}∫ \frac { 1 } { 1 +t^2 }{\rm d}t\\
&=\frac 1{\ln\frac { 2 } { 3 }}\arctan t+C\\
&=\frac 1{\ln\frac { 2 } { 3 }}\arctan \left( \frac { 2 } { 3 } \right) ^ { x }+C
\end{aligned}
$$

---

$$
\begin{aligned}
&∫ \frac { \sqrt { x ^ { 2 } + 4 x } } { x + 2 } {\rm d} x\\
&= ∫ \frac { \sqrt { ( x + 2 ) ^ { 2 } - 4 } } { x + 2 } {\rm d} x\\
&x+2=u \quad {\rm d}x={\rm d}u\\
&= ∫ \frac { \sqrt { u ^ { 2 } - 4 } } { u } {\rm d} u\\
u& = 2 \sec ( s )\quad {\rm d} u = 2 \tan ( s ) \sec ( s ) {\rm d} s \quad \sqrt { u ^ { 2 } - 4 } = \sqrt { 4 \sec ^ { 2 } ( s ) - 4 } =2 \tan ( s )\\
&= ∫ \frac {2 \tan ( s )} { 2 \sec ( s ) } 2 \tan ( s ) \sec ( s ) {\rm d} s\\
&= 2 ∫ \tan ^ { 2 } ( s ) {\rm d} s\\
&= 2 ∫ \sec ^ { 2 } ( s ) {\rm d} s - 2 ∫ 1 {\rm d} s\\
&= 2 \tan ( s ) - 2 s +C\\
&= 2 \tan \left( \sec ^ { - 1 } \left( \frac { u } { 2 } \right) \right) - 2 \sec ^ { - 1 } \left( \frac { u } { 2 } \right)+C\\
&= 2 \tan \left( \sec ^ { - 1 } \left( \frac { x+2 } { 2 } \right) \right) - 2 \sec ^ { - 1 } \left( \frac { x+2 } { 2 } \right)+C
\end{aligned}
$$

看到根号里二次式，要主动去三角换元

---

$$
\begin{aligned}
&∫ \frac {x {\rm e} ^ { x } } { \sqrt { {\rm e} ^ { x } - 1 } } {\rm d} x
\quad u = \sqrt { {\rm e} ^ { x } - 1 }\quad x=\ln(u^2+1)\quad {\rm d} u = \frac { {\rm e} ^ { x } } { 2 \sqrt { {\rm e} ^ { x } - 1 } } {\rm d} x\\
&=2∫ \frac {x {\rm e} ^ { x } } { 2\sqrt { {\rm e} ^ { x } - 1 } } {\rm d} x=2∫ { x } {\rm d} u\\
&=2 ∫ \ln \left( u ^ { 2 } + 1 \right) {\rm d} u \quad \text{integrate by part}\\
&= 2 u \ln \left( u ^ { 2 } + 1 \right) - 2 ∫ \frac { 2 u ^ { 2 } } { u ^ { 2 } + 1 } {\rm d} u\\
&= 2 u \ln \left( u ^ { 2 } + 1 \right) - 4 ∫ \left( 1 - \frac { 1 } { u ^ { 2 } + 1 } \right) {\rm d} u\\
&= 2 u \ln \left( u ^ { 2 } + 1 \right) - 4 u + 4 \tan ^ { - 1 } ( u )+C\\
&= 2x \sqrt { {\rm e} ^ { x } - 1 } - 4 \sqrt { {\rm e} ^ { x } - 1 } + 4 \tan ^ { - 1 } \left( \sqrt { {\rm e} ^ { x } - 1 } \right)+C
\end{aligned}
$$

找最复杂的求导
