---
title: 自测22
---

$$
y''+(x+{\rm e}^{2y})(y')^{3}=0
$$

变量地位互换

$$
y^{\prime \prime}=\frac{d\left(\frac{d y}{d x}\right)}{d x}=\frac{d\left(\frac{1}{x'}\right)}{d y} ⋅ \frac{d y}{d x}=\left(\frac{1}{x'}\right)'⋅ \frac{1}{x'}=\frac{-x''}{\left(x'\right)^{2}} ⋅ \frac{1}{x'}\\{}\\
-\frac{x^{\prime \prime}}{\left(x'\right)^{3}}+\left(x+{\rm e}^{2 y}\right) ⋅ \frac{1}{(x')^{3}}=0\\{}\\
x''-x={\rm e}^{2y}→ x=C_{1}{\rm e}^{y}+C_{2}{\rm e}^{-y}+\frac 13{\rm e}^{2y}
$$

---

以 $u=\frac yx$ 为新的未知函数，变换方程 $x^{2}y''-(2x+x^{2})y'+(2+x)y=0$

比较容易的思路是直接先 $\frac {\,\mathrm{d}u}{\,\mathrm{d}x},\frac{d^{2}u}{\,\mathrm{d}x^{2}}$

$$
u_{x}'=\frac{y'(x)}{x}-\frac{y(x)}{x^{2}}\\{}\\
u_{x}''=\frac{2 y(x)}{x^{3}}-\frac{2 y'(x)}{x^{2}}+\frac{y''(x)}{x}\\{}\\
x^{3}u_{x}'=x^{2} y'(x)-x y(x)\\{}\\
x^{3}u_{x}''=x^{2} y''(x)-2 x y'(x)+2 y(x)\\{}\\
x^{3}u_{x}''-x^{3}u_{x}'=0→ u_{x}''-u_{x}'=0→ u_{x}=\frac yx=C_{1}+C_{2}{\rm e}^{x}\\
y=C_{1}x+C_{2}{\rm e}^{x}x
$$

---
