---
title: 等值演算
date: 2019/09/07
---

重要式子

$$
A→ B⟺ ¬ A ∨ B
$$

>去掉 → 的式子

$$
¬ (A∧ B)⟺ ¬ A∨¬B,¬(A∨B)⟺ ¬A∧¬B
$$

>注意 ∧ ∨ 的对换

---

$$
\begin{aligned}
&(p∨q)→ (p∧r)\\
⟺& (¬ (p∨q))∨(p∧r)\\
⟺& (¬ p∧¬ q)∨(p∧r)\\
\end{aligned}
$$

已经是合取式，化为最简了。

---

用等值演算法证明

¬(p↔ q)⟺ (p∨q)∧¬(p∧q)

$$
\begin{aligned}
&¬(p↔q)\\
⟺&¬((p∧q)∨(¬p∧¬q))\\
⟺&¬(p∧q)∧¬(¬p∧¬q)\\
⟺&¬(p∧q)∧(p∨q)\\
\end{aligned}
$$

>$p↔ q⟺(p∧q)∨(¬p∧¬q)$ 定义

---

求主合取和主析取

$$
(p↔q)→ r
$$

$$
\begin{aligned}
&((p∧q)∨(¬p∧¬q))\to r\\
⟺&¬((p∧q)∨(¬p∧¬q))∨ r\\
⟺&((¬p∨¬q)∧(p∨q))∨ r\\
⟺&(¬p∨¬q∨ r)∧(p∨q∨ r)
\end{aligned}
$$

---